@prefix : <http://w3id.org/dppo/ontology/dpp-comp/> .
@prefix dcterms: <http://purl.org/dc/terms/> .
@prefix dpp-core: <http://w3id.org/dppo/ontology/dpp-core/0.1/> .
@prefix dpp-info: <http://w3id.org/dppo/ontology/dpp-info/0.1/> .
@prefix owl: <http://www.w3.org/2002/07/owl#> .
@prefix rdfs: <http://www.w3.org/2000/01/rdf-schema#> .
@prefix vann: <http://purl.org/vocab/vann/> .

: a owl:Ontology ;
    dcterms:contributor "Eva Blomqvist",
        "Huanyu Li",
        "Robin Keskisärkkä" ;
    dcterms:created "2023-11-27" ;
    dcterms:creator "Maike Jansen" ;
    dcterms:description "This is an ontology module focusing on the composition information of products." ;
    dcterms:license "https://github.com/LiUSemWeb/DPP/blob/master/LICENSE" ;
    dcterms:title "Digital Product Passport Product Composition" ;
    vann:preferredNamespacePrefix "dpp-comp" ;
    vann:preferredNamespaceUri "http://w3id.org/dppo/ontology/dpp-comp/" ;
    rdfs:seeAlso <https://github.com/LiUSemWeb/DPPO> ;
    owl:imports dpp-core:,
        dpp-info: ;
    owl:versionIRI <http://w3id.org/dppo/ontology/dpp-comp/0.1/> ;
    owl:versionInfo "0.1" .

:SubstanceHinderingRecycling a owl:Class ;
    rdfs:label "Substance findering recycling"@en ;
    rdfs:comment "A substance that hinders recycling of a product."@en ;
    rdfs:subClassOf :SubstanceOfConcern .

:ToxicSubstance a owl:Class ;
    rdfs:label "Toxic substance"@en ;
    rdfs:comment "A toxic substance."@en ;
    rdfs:subClassOf :SubstanceOfConcern .

:aboutPart a owl:ObjectProperty ;
    rdfs:label "about part"@en ;
    rdfs:comment "Relation between the piece of information representing the composition, and the part involved in the relation."@en ;
    rdfs:domain dpp-info:CompositionInformation ;
    rdfs:range <http://w3id.org/dppo/ontology/dpp-odp/Product> ;
    rdfs:subPropertyOf dpp-info:isAbout .

:aboutWhole a owl:ObjectProperty ;
    rdfs:label "about whole"@en ;
    rdfs:comment "Relation between the piece of information representing the composition, and the whole involved in the relation."@en ;
    rdfs:domain dpp-info:CompositionInformation ;
    rdfs:range <http://w3id.org/dppo/ontology/dpp-odp/Product> ;
    rdfs:subPropertyOf dpp-info:isAbout ;
    owl:inverseOf dpp-info:hasCompositionInformation .

dpp-info:hasCompositionInformation a owl:ObjectProperty .

:SubstanceOfConcern a owl:Class ;
    rdfs:label "Substance of Concern"@en ;
    rdfs:comment "Substance of concern as defined in the ESPR, meaning it is a substance that is either toxic or something that hinders recycling of the product."@en ;
    rdfs:subClassOf <http://w3id.org/dppo/ontology/dpp-core/Substance> .

dpp-info:CompositionInformation a owl:Class .

dpp-info:isAbout a owl:ObjectProperty .

