<?xml version="1.0" encoding="utf-8"?>
<rdf:RDF
   xmlns:dcterms="http://purl.org/dc/terms/"
   xmlns:owl="http://www.w3.org/2002/07/owl#"
   xmlns:rdf="http://www.w3.org/1999/02/22-rdf-syntax-ns#"
   xmlns:rdfs="http://www.w3.org/2000/01/rdf-schema#"
   xmlns:vann="http://purl.org/vocab/vann/"
>
  <rdf:Description rdf:about="http://w3id.org/dppo/ontology/dpp-comp/">
    <rdf:type rdf:resource="http://www.w3.org/2002/07/owl#Ontology"/>
    <owl:versionIRI rdf:resource="http://w3id.org/dppo/ontology/dpp-comp/0.1/"/>
    <owl:imports rdf:resource="http://w3id.org/dppo/ontology/dpp-core/0.1/"/>
    <owl:imports rdf:resource="http://w3id.org/dppo/ontology/dpp-info/0.1/"/>
    <dcterms:contributor>Eva Blomqvist</dcterms:contributor>
    <dcterms:contributor>Huanyu Li</dcterms:contributor>
    <dcterms:contributor>Robin Keskisärkkä</dcterms:contributor>
    <dcterms:created>2023-11-27</dcterms:created>
    <dcterms:creator>Maike Jansen</dcterms:creator>
    <dcterms:description>This is an ontology module focusing on the composition information of products.</dcterms:description>
    <dcterms:license>https://github.com/LiUSemWeb/DPP/blob/master/LICENSE</dcterms:license>
    <dcterms:title>Digital Product Passport Product Composition</dcterms:title>
    <vann:preferredNamespacePrefix>dpp-comp</vann:preferredNamespacePrefix>
    <vann:preferredNamespaceUri>http://w3id.org/dppo/ontology/dpp-comp/</vann:preferredNamespaceUri>
    <rdfs:seeAlso rdf:resource="https://github.com/LiUSemWeb/DPPO"/>
    <owl:versionInfo>0.1</owl:versionInfo>
  </rdf:Description>
  <rdf:Description rdf:about="http://w3id.org/dppo/ontology/dpp-info/0.1/hasCompositionInformation">
    <rdf:type rdf:resource="http://www.w3.org/2002/07/owl#ObjectProperty"/>
  </rdf:Description>
  <rdf:Description rdf:about="http://w3id.org/dppo/ontology/dpp-comp/ToxicSubstance">
    <rdf:type rdf:resource="http://www.w3.org/2002/07/owl#Class"/>
    <rdfs:subClassOf rdf:resource="http://w3id.org/dppo/ontology/dpp-comp/SubstanceOfConcern"/>
    <rdfs:comment xml:lang="en">A toxic substance.</rdfs:comment>
    <rdfs:label xml:lang="en">Toxic substance</rdfs:label>
  </rdf:Description>
  <rdf:Description rdf:about="http://w3id.org/dppo/ontology/dpp-comp/aboutPart">
    <rdf:type rdf:resource="http://www.w3.org/2002/07/owl#ObjectProperty"/>
    <rdfs:subPropertyOf rdf:resource="http://w3id.org/dppo/ontology/dpp-info/0.1/isAbout"/>
    <rdfs:domain rdf:resource="http://w3id.org/dppo/ontology/dpp-info/0.1/CompositionInformation"/>
    <rdfs:range rdf:resource="http://w3id.org/dppo/ontology/dpp-odp/Product"/>
    <rdfs:comment xml:lang="en">Relation between the piece of information representing the composition, and the part involved in the relation.</rdfs:comment>
    <rdfs:label xml:lang="en">about part</rdfs:label>
  </rdf:Description>
  <rdf:Description rdf:about="http://w3id.org/dppo/ontology/dpp-comp/aboutWhole">
    <rdf:type rdf:resource="http://www.w3.org/2002/07/owl#ObjectProperty"/>
    <rdfs:subPropertyOf rdf:resource="http://w3id.org/dppo/ontology/dpp-info/0.1/isAbout"/>
    <owl:inverseOf rdf:resource="http://w3id.org/dppo/ontology/dpp-info/0.1/hasCompositionInformation"/>
    <rdfs:domain rdf:resource="http://w3id.org/dppo/ontology/dpp-info/0.1/CompositionInformation"/>
    <rdfs:range rdf:resource="http://w3id.org/dppo/ontology/dpp-odp/Product"/>
    <rdfs:comment xml:lang="en">Relation between the piece of information representing the composition, and the whole involved in the relation.</rdfs:comment>
    <rdfs:label xml:lang="en">about whole</rdfs:label>
  </rdf:Description>
  <rdf:Description rdf:about="http://w3id.org/dppo/ontology/dpp-comp/SubstanceHinderingRecycling">
    <rdf:type rdf:resource="http://www.w3.org/2002/07/owl#Class"/>
    <rdfs:subClassOf rdf:resource="http://w3id.org/dppo/ontology/dpp-comp/SubstanceOfConcern"/>
    <rdfs:comment xml:lang="en">A substance that hinders recycling of a product.</rdfs:comment>
    <rdfs:label xml:lang="en">Substance findering recycling</rdfs:label>
  </rdf:Description>
  <rdf:Description rdf:about="http://w3id.org/dppo/ontology/dpp-comp/SubstanceOfConcern">
    <rdf:type rdf:resource="http://www.w3.org/2002/07/owl#Class"/>
    <rdfs:subClassOf rdf:resource="http://w3id.org/dppo/ontology/dpp-core/Substance"/>
    <rdfs:comment xml:lang="en">Substance of concern as defined in the ESPR, meaning it is a substance that is either toxic or something that hinders recycling of the product.</rdfs:comment>
    <rdfs:label xml:lang="en">Substance of Concern</rdfs:label>
  </rdf:Description>
  <rdf:Description rdf:about="http://w3id.org/dppo/ontology/dpp-info/0.1/isAbout">
    <rdf:type rdf:resource="http://www.w3.org/2002/07/owl#ObjectProperty"/>
  </rdf:Description>
  <rdf:Description rdf:about="http://w3id.org/dppo/ontology/dpp-info/0.1/CompositionInformation">
    <rdf:type rdf:resource="http://www.w3.org/2002/07/owl#Class"/>
  </rdf:Description>
</rdf:RDF>
